new/generatedproof/sync.v
@@ -557,5 +557,81 @@ Global Instance wp_func_call_runtime_Semrelease :
   WpFuncCall sync.runtime_Semrelease _ (is_pkg_defined sync) :=
   ltac:(solve_wp_func_call).
 
+Global Instance wp_method_call_Cond'ptr_Broadcast :
+  WpMethodCall (ptrT.id sync.Cond.id) "Broadcast" _ (is_pkg_defined sync) :=
+  ltac:(solve_wp_method_call).
+
+Global Instance wp_method_call_Cond'ptr_Signal :
+  WpMethodCall (ptrT.id sync.Cond.id) "Signal" _ (is_pkg_defined sync) :=
+  ltac:(solve_wp_method_call).
+
+Global Instance wp_method_call_Cond'ptr_Wait :
+  WpMethodCall (ptrT.id sync.Cond.id) "Wait" _ (is_pkg_defined sync) :=
+  ltac:(solve_wp_method_call).
+
+Global Instance wp_method_call_Mutex'ptr_Lock :
+  WpMethodCall (ptrT.id sync.Mutex.id) "Lock" _ (is_pkg_defined sync) :=
+  ltac:(solve_wp_method_call).
+
+Global Instance wp_method_call_Mutex'ptr_TryLock :
+  WpMethodCall (ptrT.id sync.Mutex.id) "TryLock" _ (is_pkg_defined sync) :=
+  ltac:(solve_wp_method_call).
+
+Global Instance wp_method_call_Mutex'ptr_Unlock :
+  WpMethodCall (ptrT.id sync.Mutex.id) "Unlock" _ (is_pkg_defined sync) :=
+  ltac:(solve_wp_method_call).
+
+Global Instance wp_method_call_Once'ptr_Do :
+  WpMethodCall (ptrT.id sync.Once.id) "Do" _ (is_pkg_defined sync) :=
+  ltac:(solve_wp_method_call).
+
+Global Instance wp_method_call_Once'ptr_doSlow :
+  WpMethodCall (ptrT.id sync.Once.id) "doSlow" _ (is_pkg_defined sync) :=
+  ltac:(solve_wp_method_call).
+
+Global Instance wp_method_call_RWMutex'ptr_Lock :
+  WpMethodCall (ptrT.id sync.RWMutex.id) "Lock" _ (is_pkg_defined sync) :=
+  ltac:(solve_wp_method_call).
+
+Global Instance wp_method_call_RWMutex'ptr_RLock :
+  WpMethodCall (ptrT.id sync.RWMutex.id) "RLock" _ (is_pkg_defined sync) :=
+  ltac:(solve_wp_method_call).
+
+Global Instance wp_method_call_RWMutex'ptr_RLocker :
+  WpMethodCall (ptrT.id sync.RWMutex.id) "RLocker" _ (is_pkg_defined sync) :=
+  ltac:(solve_wp_method_call).
+
+Global Instance wp_method_call_RWMutex'ptr_RUnlock :
+  WpMethodCall (ptrT.id sync.RWMutex.id) "RUnlock" _ (is_pkg_defined sync) :=
+  ltac:(solve_wp_method_call).
+
+Global Instance wp_method_call_RWMutex'ptr_TryLock :
+  WpMethodCall (ptrT.id sync.RWMutex.id) "TryLock" _ (is_pkg_defined sync) :=
+  ltac:(solve_wp_method_call).
+
+Global Instance wp_method_call_RWMutex'ptr_TryRLock :
+  WpMethodCall (ptrT.id sync.RWMutex.id) "TryRLock" _ (is_pkg_defined sync) :=
+  ltac:(solve_wp_method_call).
+
+Global Instance wp_method_call_RWMutex'ptr_Unlock :
+  WpMethodCall (ptrT.id sync.RWMutex.id) "Unlock" _ (is_pkg_defined sync) :=
+  ltac:(solve_wp_method_call).
+
+Global Instance wp_method_call_RWMutex'ptr_rUnlockSlow :
+  WpMethodCall (ptrT.id sync.RWMutex.id) "rUnlockSlow" _ (is_pkg_defined sync) :=
+  ltac:(solve_wp_method_call).
+
+Global Instance wp_method_call_WaitGroup'ptr_Add :
+  WpMethodCall (ptrT.id sync.WaitGroup.id) "Add" _ (is_pkg_defined sync) :=
+  ltac:(solve_wp_method_call).
+
+Global Instance wp_method_call_WaitGroup'ptr_Done :
+  WpMethodCall (ptrT.id sync.WaitGroup.id) "Done" _ (is_pkg_defined sync) :=
+  ltac:(solve_wp_method_call).
+
+Global Instance wp_method_call_WaitGroup'ptr_Wait :
+  WpMethodCall (ptrT.id sync.WaitGroup.id) "Wait" _ (is_pkg_defined sync) :=
+  ltac:(solve_wp_method_call).
+
 End names.
 End sync.
